Gave skolemized definition of exponentials and proven they're unique (the proof is nicer now). Gave alternative definition of has_exponentials with curry. Proved that setoids have exponentials using this new definition. Proved that CoqSet and CoqSetoid are cartesian closed.

Exponential.v
@@ -13,6 +13,13 @@ Definition exponential {C : Cat} {hp : has_products C}
     forall (Z : Ob C) (e : Hom (prodOb Z X) Y),
       exists!! u : Hom Z E, ProductFunctor_fmap u (id X) .> eval == e.
 
+Definition exponential_skolem {C : Cat} {hp : has_products C}
+  (X Y E : Ob C) (eval : Hom (prodOb E X) Y)
+  (curry : forall E' : Ob C, Hom (prodOb E' X) Y -> Hom E' E) : Prop :=
+    forall (E' : Ob C) (eval' : Hom (prodOb E' X) Y),
+      setoid_unique (fun u : Hom E' E =>
+        ProductFunctor_fmap u (id X) .> eval == eval') (curry E' eval').
+
 Theorem exponential_unique :
     forall (C : Cat) (hp : has_products C) (X Y : Ob C)
     (E : Ob C) (eval : Hom (prodOb E X) Y)
@@ -44,6 +51,37 @@ Proof.
           rewrite H2 in Hu'1. assumption.
 Defined.
 
+Theorem exponential_skolem_unique_long :
+    forall (C : Cat) (hp : has_products C) (X Y : Ob C)
+    (E : Ob C) (eval : Hom (prodOb E X) Y)
+      (curry : forall Z : Ob C, Hom (prodOb Z X) Y -> Hom Z E)
+    (E' : Ob C) (eval' : Hom (prodOb E' X) Y)
+      (curry' : forall Z : Ob C, Hom (prodOb Z X) Y -> Hom Z E'),
+        exponential_skolem X Y E eval curry ->
+        exponential_skolem X Y E' eval' curry'
+        -> E ~ E'.
+Proof.
+  intros. red. do 2 red in H. do 2 red in H0.
+  exists (curry' E eval). red. exists (curry E' eval').
+  split.
+    destruct (H E eval) as [H1 H2].
+      rewrite <- (H2 (curry' E eval .> curry E' eval')).
+        rewrite (H2 (id E)).
+          reflexivity.
+          rewrite ProductFunctor_fmap_pres_id, id_left. reflexivity.
+        rewrite ProductFunctor_fmap_pres_comp_l.
+          destruct (H E' eval'), (H0 E eval).
+            rewrite comp_assoc. rewrite H3. rewrite H5. reflexivity.
+    destruct (H0 E' eval') as [H1 H2].
+      rewrite <- (H2 (curry E' eval' .> curry' E eval)).
+        rewrite (H2 (id E')).
+          reflexivity.
+          rewrite ProductFunctor_fmap_pres_id, id_left. reflexivity.
+        rewrite ProductFunctor_fmap_pres_comp_l.
+          destruct (H E' eval'), (H0 E eval).
+            rewrite comp_assoc. rewrite H5. rewrite H3. reflexivity.
+Qed.
+
 Class has_exponentials (C : Cat) {hp : has_products C} : Type :=
 {
     expOb : Ob C -> Ob C -> Ob C;
@@ -51,4 +89,15 @@ Class has_exponentials (C : Cat) {hp : has_products C} : Type :=
       Hom (prodOb (expOb X Y) X) Y;
     is_exponential : forall (X Y : Ob C),
       exponential X Y (expOb X Y) (eval X Y)
+}.
+
+Class has_exponentials' (C : Cat) {hp : has_products C} : Type :=
+{
+    expOb' : Ob C -> Ob C -> Ob C;
+    eval' : forall X Y : Ob C,
+      Hom (prodOb (expOb' X Y) X) Y;
+    curry' : forall {X Y Z : Ob C},
+      Hom (prodOb Z X) Y -> Hom Z (expOb' X Y);
+    is_exponential' : forall (X Y : Ob C),
+      exponential_skolem X Y (expOb' X Y) (eval' X Y) (@curry' X Y)
 }.
